{"nbformat":4,"nbformat_minor":0,"metadata":{"colab":{"name":"2022_04_22.ipynb","provenance":[],"collapsed_sections":["rCz1kHnvvqQs","F7FrfTILol-7","VtxI1d3gsVwc","ECo2PV5wvYkC","D-zNY0iZv_ln"],"authorship_tag":"ABX9TyPQ8WjqVASYWGVn2lKBUT4s"},"kernelspec":{"name":"python3","display_name":"Python 3"},"language_info":{"name":"python"}},"cells":[{"cell_type":"code","source":["import numpy as np\n","import matplotlib.pyplot as plt"],"metadata":{"id":"QjL6s9mUn-DY"},"execution_count":null,"outputs":[]},{"cell_type":"markdown","source":["# Lecture 30-VMLS left & right inv."],"metadata":{"id":"0cSclX0GnxhS"}},{"cell_type":"markdown","source":["## Left and right inverses"],"metadata":{"id":"rCz1kHnvvqQs"}},{"cell_type":"code","source":["A = np.array([[-3,-4],\n","              [ 4, 6],\n","              [ 1, 1]])\n","\n","B = np.array([[-11,-10, 16],\n","              [  7,  8,-11]]) * (1/9)\n","\n","C = np.array([[ 0,-1, 6],\n","              [ 0, 1,-4]]) * (1/2)"],"metadata":{"id":"FZGukUZ3n6SE"},"execution_count":null,"outputs":[]},{"cell_type":"code","source":["print(f\"BA = I: \\n{np.round(np.dot(B, A),4)}\")\n","print(f\"CA = I: \\n{np.round(np.dot(C, A),4)}\")"],"metadata":{"colab":{"base_uri":"https://localhost:8080/"},"id":"MHHQgG25oX7j","executionInfo":{"status":"ok","timestamp":1650765270441,"user_tz":-540,"elapsed":8,"user":{"displayName":"이도훈","userId":"08244818386454187914"}},"outputId":"da999aa6-df52-4b96-c0f1-8e03975ec708"},"execution_count":null,"outputs":[{"output_type":"stream","name":"stdout","text":["BA = I: \n","[[ 1. -0.]\n"," [ 0.  1.]]\n","CA = I: \n","[[1. 0.]\n"," [0. 1.]]\n"]}]},{"cell_type":"markdown","source":["### left inverse: $XA = I$\n","If a matrix has a left inverse, than that matrix's columns are linearly independent.\n","\n","Because: if $Ax = 0$ and $CA = I$ then,  \n","$\\qquad0 = C0 = C(Ax) = (CA)x = Ix = x$...\n","\n","And, __a matrix is left-invertible if and only if its columns are linearly independent.__\n","which also, left-invertible matrices are tall or square."],"metadata":{"id":"F7FrfTILol-7"}},{"cell_type":"markdown","source":["suppose $Ax = b$, and A has a left inverse C\n","\n","then $Cb = C(Ax) = (CA)x = Ix = x$\n","\n","its like if $ax = b$ then $x = {b \\over a}$."],"metadata":{"id":"waNPmuF1p-GN"}},{"cell_type":"code","source":["b = np.array([ 1,-2, 0])\n","\n","print(f\"solution 1, Bb: x = {np.dot(B, b)}\")\n","print(f\"solution 2, Cb: x = {np.dot(C, b)}\")"],"metadata":{"colab":{"base_uri":"https://localhost:8080/"},"id":"Y7Tj8w0OrmaW","executionInfo":{"status":"ok","timestamp":1650765270441,"user_tz":-540,"elapsed":6,"user":{"displayName":"이도훈","userId":"08244818386454187914"}},"outputId":"5a9ea699-c86d-4dd2-8e50-bea99fa542df"},"execution_count":null,"outputs":[{"output_type":"stream","name":"stdout","text":["solution 1, Bb: x = [ 1. -1.]\n","solution 2, Cb: x = [ 1. -1.]\n"]}]},{"cell_type":"markdown","source":["### right inverse: $AX = I$\n","If a matrix has a right inverse, than that matrix's rows are linearly independent.\n","\n","suppose A has a right inverse B\n","\n","for the equations $Ax = b$, $x = Bb$ is a solution.\n","\n","Because: $Ax = A(Bb) = (AB)b = Ib = I$"],"metadata":{"id":"VtxI1d3gsVwc"}},{"cell_type":"markdown","source":["If $B$,$C$ are left inverse of $A$, then $B^T$, $C^T$ are right inverse of $A^T$"],"metadata":{"id":"QsjyAcT4uPuI"}},{"cell_type":"code","source":["## A.T@x = (1,2)\n","b = np.array([1,2])\n","print(f\"solution 1: {np.dot(B.T, b)}\")\n","print(f\"solution 2: {np.dot(C.T, b)}\")"],"metadata":{"colab":{"base_uri":"https://localhost:8080/"},"id":"uakcQSEQu0q7","executionInfo":{"status":"ok","timestamp":1650765270442,"user_tz":-540,"elapsed":5,"user":{"displayName":"이도훈","userId":"08244818386454187914"}},"outputId":"b8e38dca-5641-40a3-fe80-dd8c67b1c88b"},"execution_count":null,"outputs":[{"output_type":"stream","name":"stdout","text":["solution 1: [ 0.33333333  0.66666667 -0.66666667]\n","solution 2: [ 0.   0.5 -1. ]\n"]}]},{"cell_type":"markdown","source":["## Inverse"],"metadata":{"id":"ECo2PV5wvYkC"}},{"cell_type":"markdown","source":["if A has a left and a right inverse, they are unique and equal, so A must be square\n","\n","if $AX = I$, $YA = I$\n","\n","$\\qquad X = IX = (YA)X = Y(AX) = YI = Y$\n","\n","we donote them by $A^{-1}$"],"metadata":{"id":"I1IKQOuzwDFH"}},{"cell_type":"markdown","source":["suppose A is invertible\n","\n","for any b, $Ax = b$ has the unique solution\n","\n","$\\qquad x = A^{-1}b$\n","\n","simple-looking formula $x = A^{-1}b$ is basis for many applications"],"metadata":{"id":"nzNGO7rnw-Ng"}},{"cell_type":"markdown","source":["### Examples\n","\n","1. $I^{-1} = I$\n","2. if Q is orthogonal and square with $Q^TQ = I$, then $Q^{-1} = Q^T$ and also $QQ^T = I$\n","3. $2 \\times 2$ matrix A is invertible if and only $A_{11}A_{22} \\ne A_{12}A_{21}$\n","$\\qquad A_{-1} = {1 \\over A_{11}A_{22} - A_{12}A_{21}}\n","\\begin{bmatrix}\n","A_{22} \\quad\n","-A_{12} \\\\\n","-A_{21} \\quad\n","A_{11}\n","\\end{bmatrix}$"],"metadata":{"id":"Kok9kfF1R1SD"}},{"cell_type":"markdown","source":["### Properties\n","\n","> $(AB)^{-1} = b^{-1}A^{-1}$ (provided inverses exist)\n","\n","> $(A^T)^{-1} = (A^{-1})^T$ (sometimes denoted $A^{-T}$)\n","\n","> negative matrix powers: $(A^{-1})^k$ is denoted $A^{-k}$\n","\n","> with $A^0 = I$, identity $A^kA^l = A^{k+l}$ holds for any integers $k, l$"],"metadata":{"id":"gbG1TPJfU0WE"}},{"cell_type":"markdown","source":["## Pseudo-inverse"],"metadata":{"id":"D-zNY0iZv_ln"}},{"cell_type":"markdown","source":["### Invertibility of Gram matrix\n","\n","A has linearly indenpendent columns if and only if $A^TA$ is invertible<br>\n","to see this, we'll show that $Ax = 0 \\Leftrightarrow A^TAx = 0$<br>\n","$\\Rightarrow$: if $Ax = 0$ then $(A^TA)x = A^T(Ax) = A^T0 = 0$<br>\n","$\\Leftarrow$: if $A^TAx = 0$ then <br>\n","$\\qquad 0 = x^T(A^TAx) = (Ax)^T(Ax) = \n","\\begin{Vmatrix}\n","Ax\n","\\end{Vmatrix}^2\n","= 0$<br>\n","so Ax = 0"],"metadata":{"id":"YRHSCG2fwCE4"}},{"cell_type":"markdown","source":["### Pseudo-inverse of tall matrix\n","\n","the pseudo-inverse of A with independent columns is<br>\n","$\\qquad A^{\\dagger} = (A^TA)^{-1}A^T$<br>\n","it is a left inverse of A:<br>\n","$\\qquad A^{\\dagger}A = (A^TA)^{-1}A^TA = (A^TA)^{-1}(A^TA) = I$<br>\n","reduces to $A^{-1}$ when $A$ is square:<br>\n","$\\qquad A^{\\dagger} = (A^TA)^{-1}A^T = A^{-1}A^{-T}A^T = A^{-1}I = A^{-1}$"],"metadata":{"id":"gfAI87peKDhA"}},{"cell_type":"markdown","source":["### pseudo-inverse of wide matrix\n","if $A$ is wide, with linearly independent rows, $AA^T$ is invertible<br>\n","pseudo-inverse is defined as<br>\n","$\\qquad A^{\\dagger} = A^T(AA^T)^{-1}$<br>\n","$A^{\\dagger}$ is a right inverse of A:<br>\n","$\\qquad AA^{\\dagger} = AA^T(AA^T)^{-1} = I$<br>\n","reduces to $A^{-1}$ when $A$ is square:<br>\n","$\\qquad A^T(AA^T)^{-1} = A^TA^{-T}A^{-1} = A^{-1}$"],"metadata":{"id":"VrUOCgv0MoxV"}},{"cell_type":"markdown","source":["### Pseudo-inverse via QR factorization\n","suppose A has linearly independent columns, $A = QR$<br>\n","then $A^TA = (QR)^T(QR) = R^TQ^TQR = R^TR$<br>\n","so<br> \n","$\\qquad A^{\\dagger} = (A^TA)^{-1}A^T = (R^TR)^{-1}(QR)^T = R^{-1}R^{-T}R^TQ^T = R^{-1}Q^T$<br>\n","can compute $A^{\\dagger}$ using back substitution on columns of $Q^T$<br>\n","for A with linearly indenpendent rows, $A^{\\dagger} = QR^{-T}$"],"metadata":{"id":"oV2PvwYYNaWP"}}]}